testdata/cue/definitions/bug29_named_multiconjunct_conflict_bottoms.cue
@@ -1,0 +1,3 @@
+#Base: {#name: string, val: 1}
+#LS: #Base & {#extra: "x"}
+out: #LS & {#name: "n", val: 2}
