testdata/cue/definitions/bug29_named_multiconjunct_def_narrowed.cue
@@ -1,0 +1,3 @@
+#Base: {#name: string, vis: #name}
+#LS: #Base & {#extra: "x"}
+out: #LS & {#name: "argocd-ls"}
