testdata/cue/definitions/bug29_nested_named_multiconjunct_narrowed.cue
@@ -1,0 +1,4 @@
+#A: {#name: string, vis: #name}
+#B: #A & {#p: "b"}
+#C: #B & {#q: "c"}
+out: #C & {#name: "deep"}
